pulse/ulib/experimental/Steel.Reference.fsti
@@ -1,52 +1,66 @@
 module Steel.Reference
+
 open Steel.Effect
 open Steel.Effect.Atomic
 open Steel.Memory
 open FStar.Ghost
+module U = FStar.Universe
+module A = Steel.Actions
+
+#set-options "--print_universes --print_implicits"
 
 let perm = p:perm{readable p}
 let full : perm = full_perm
 let trivial_preorder #a : Preorder.preorder a = fun _ _ -> True
-let ref (a:Type0) = reference a trivial_preorder
-let is_ref (#a:Type0) (r:ref a) (p:perm) = ref_perm r p
-let pts_to (#a:Type0) (r:ref a) (p:perm) (v:erased a) : hprop = pts_to_ref r p v
+let ref (a:Type u#0) = reference (U.raise_t u#0 u#1 a) trivial_preorder
+let ref_pre (a: Type u#0) (pre: Preorder.preorder a) = reference (U.raise_t u#0 u#1 a) (A.raise_preorder pre)
+let is_ref (#a:Type u#0) (r:ref a) (p:perm) : hprop u#1 = ref_perm r p
+let pts_to (#a:Type u#0) (r:ref a) (p:perm) (v:erased a) : hprop u#1 =
+  pts_to_ref r p (U.raise_val (reveal v))
+let pts_to_pre (#a:Type u#0) (#pre: Preorder.preorder a) (r:ref_pre a pre) (p:perm) (v:erased a) : hprop u#1 =
+  pts_to_ref r p (U.raise_val (reveal v))
+let h_exists (#a:Type u#0) (f: (a -> hprop u#1)) : hprop u#1 =
+  h_exists #(U.raise_t u#0 u#1 a) (fun x -> f (U.downgrade_val x))
 
-val alloc (#a:Type) (x:a)
+
+val alloc (#a:Type0) (x:a)
   : SteelT (ref a) emp (fun r -> pts_to r full x)
 
-val read (#a:Type) (#p:perm) (#v:erased a) (r:ref a)
+val read (#a:Type0) (#p:perm) (#v:erased a) (r:ref a)
   : SteelT a (pts_to r p v) (fun x -> pts_to r p x)
 
-val read_refine (#a:Type) (#p:perm) (q:a -> hprop) (r:ref a)
+val read_refine (#a:Type0) (#p:perm) (q:a -> hprop) (r:ref a)
   : SteelT a (h_exists (fun (v:a) -> pts_to r p v `star` q v))
              (fun v -> pts_to r p v `star` q v)
 
-val write (#a:Type) (#v:erased a) (r:ref a) (x:a)
+val write (#a:Type0) (#v:erased a) (r:ref a) (x:a)
   : SteelT unit (pts_to r full v) (fun _ -> pts_to r full x)
 
-val free (#a:Type) (#v:erased a) (r:ref a)
+val free (#a:Type0) (#v:erased a) (r:ref a)
   : SteelT unit (pts_to r full v) (fun _ -> emp)
 
-val share (#a:Type) (#p:perm) (#v:erased a) (r:ref a)
+val share (#a:Type0) (#p:perm) (#v:erased a) (r:ref a)
   : SteelT unit
     (pts_to r p v)
     (fun _ -> pts_to r (half_perm p) v `star` pts_to r (half_perm p) v)
 
-val gather (#a:Type) (#p0:perm) (#p1:perm) (#v0 #v1:erased a) (r:ref a)
+val gather (#a:Type0) (#p0:perm) (#p1:perm) (#v0 #v1:erased a) (r:ref a)
   : SteelT unit
     (pts_to r p0 v0 `star` pts_to r p1 v1)
     (fun _ -> pts_to r (sum_perm p0 p1) v0)
 
-val ghost_read (#a:Type) (#uses:Set.set lock_addr) (#p:perm) (#v:Ghost.erased a) (r:ref a)
+val ghost_read (#a:Type0) (#uses:Set.set lock_addr) (#p:perm) (#v:Ghost.erased a) (r:ref a)
   : SteelAtomic a uses true
     (pts_to r p v)
     (fun x -> pts_to r p x)
 
-val ghost_read_refine (#a:Type) (#uses:Set.set lock_addr) (#p:perm) (r:ref a)
+val ghost_read_refine (#a:Type0) (#uses:Set.set lock_addr) (#p:perm) (r:ref a)
   (q:a -> hprop)
   : SteelAtomic a uses true
     (h_exists (fun (v:a) -> pts_to r p v `star` q v))
     (fun v -> pts_to r p v `star` q v)
+
+module U = FStar.Universe
 
 val cas
   (#t:eqtype)
@@ -64,36 +78,54 @@ val cas
 
 ////////////////////////////////////////////////////////////////////////////////
 
-val alloc_monotonic_ref (#a:Type) (p:Preorder.preorder a) (v:a)
-  : SteelT (reference a p) emp (fun r -> pts_to_ref r full v)
+val alloc_monotonic_ref (#a:Type0) (p:Preorder.preorder a) (v:a)
+  : SteelT (ref_pre a p) emp (fun r -> pts_to_pre r full v)
 
-val read_monotonic_ref (#a:Type) (#q:perm) (#p:Preorder.preorder a) (#frame:a -> hprop)
-                       (r:reference a p)
-  : SteelT a (h_exists (fun (v:a) -> pts_to_ref r q v `star` frame v))
-             (fun v -> pts_to_ref r q v `star` frame v)
+val read_monotonic_ref
+  (#a:Type0)
+  (#q:perm)
+  (#p:Preorder.preorder a)
+  (#frame:a -> hprop)
+  (r:ref_pre a p)
+  : SteelT a (h_exists (fun (v:a) ->
+                pts_to_pre r q v `star` frame v))
+             (fun v -> pts_to_pre r q v `star` frame v)
 
-val write_monotonic_ref (#a:Type) (#p:Preorder.preorder a) (#v:erased a)
-                       (r:reference a p) (x:a{p v x})
-  : SteelT unit (pts_to_ref r full v)
-                (fun v -> pts_to_ref r full x)
+val write_monotonic_ref
+  (#a:Type0)
+  (#p:Preorder.preorder a)
+  (#v:erased a)
+  (r:ref_pre a p)
+  (x:a{p v x})
+  : SteelT unit
+    (pts_to_pre r full v)
+    (fun v -> pts_to_pre r full x)
 
 val pure (p:prop) : hprop
 
 let property (a:Type) = a -> prop
 
-val witnessed (#a:Type) (#p:Preorder.preorder a) (r:reference a p)
-              (fact:property a) : prop
+val witnessed
+  (#a:Type0)
+  (#p:Preorder.preorder a)
+  (r:ref_pre a p)
+  (fact:property a) : prop
 
-let stable_property (#a:Type) (p:Preorder.preorder a) = fact:property a { Preorder.stable fact p }
+let stable_property (#a:Type0) (p:Preorder.preorder a) = fact:property a { Preorder.stable fact p }
 
-val witness (#a:Type) (#q:perm) (#p:Preorder.preorder a) (r:reference a p)
-            (fact:stable_property p)
-            (v:(Ghost.erased a))
-            (_:squash (fact v))
-  : SteelT unit (pts_to_ref r q v)
-                (fun _ -> pts_to_ref r q v `star` pure (witnessed r fact))
+val witness
+  (#a:Type0)
+  (#q:perm)
+  (#p:Preorder.preorder a)
+  (r:ref_pre a p)
+  (fact:stable_property p)
+  (v:(Ghost.erased a))
+  (_:squash (fact v))
+  : SteelT unit
+    (pts_to_pre r q v)
+    (fun _ -> pts_to_pre r q v `star` pure (witnessed r fact))
 
-val recall (#a:Type) (#q:perm) (#p:Preorder.preorder a) (#fact:property a)
-           (r:reference a p) (v:(Ghost.erased a))
-  : SteelT unit (pts_to_ref r q v `star` pure (witnessed r fact))
-                (fun _ -> pts_to_ref r q v `star` pure (fact v))
+val recall (#a:Type0) (#q:perm) (#p:Preorder.preorder a) (#fact:property a)
+           (r:ref_pre a p) (v:(Ghost.erased a))
+  : SteelT unit (pts_to_pre r q v `star` pure (witnessed r fact))
+                (fun _ -> pts_to_pre r q v `star` pure (fact v))
